src/program_proof/tulip/program/gcoord/gcoord_prepare.v
@@ -10,7 +10,9 @@ Section program.
     (gcoord : loc) (tsW : u64) (pwrsP : loc) (ptgsP : Slice.t)
     (pwrs : dbmap) (ptgs : txnptgs) gid γ :
     let ts := uint.nat tsW in
+    is_lnrz_tid γ ts -∗
     safe_txn_pwrs γ gid ts pwrs -∗
+    safe_txn_ptgs γ ts ptgs -∗
     own_map pwrsP DfracDiscarded pwrs -∗
     is_txnptgs_in_slice ptgsP ptgs -∗
     is_gcoord gcoord gid γ -∗
@@ -20,7 +22,7 @@ Section program.
         if valid then safe_group_txnphase γ ts gid phase else True
     }}}.
   Proof.
-    iIntros (ts) "#Hsafepwrs #Hpwrs #Hptgs #Hgcoord".
+    iIntros (ts) "#Hlnrz #Hsafepwrs #Hsafeptgs #Hpwrs #Hptgs #Hgcoord".
     iIntros (Φ) "!> _ HΦ".
     wp_rec.
 
@@ -44,7 +46,8 @@ Section program.
       iAssert (is_gcoord_with_addrm gcoord gid addrm γ)%I as "#Hgcoord".
       { iFrame "HcvP # %". }
       wp_apply wp_fork.
-      { wp_apply (wp_GroupCoordinator__PrepareSession with "Hsafepwrs Hpwrs Hptgs Hgcoord").
+      { wp_apply (wp_GroupCoordinator__PrepareSession
+                   with "Hlnrz Hsafepwrs Hsafeptgs Hpwrs Hptgs Hgcoord").
         { by apply elem_of_dom_2 in Hrid. }
         done.
       }
