src/program_proof/tulip/program/replica/replica_apply_abort.v
@@ -231,8 +231,11 @@ Section program.
         assert (ts' = ts) as -> by word.
         apply Hcpmts.
       }
-      iClear "Hrpvds".
+      iDestruct (big_sepS_delete_affine _ _ ts with "Hlnrzs") as "Hlnrzs'".
+      iDestruct (big_sepM_delete_affine _ _ ts with "Hsafebk") as "Hsafebk'".
+      iClear "Hrpvds Hlnrzs Hsafebk".
       iFrame "∗ # %".
+      rewrite !dom_delete_L. iFrame "#".
       iPureIntro. simpl.
       exists (<[ts := false]> cm).
       split.
